Group Thy/Basics.v
@@ -1,0 +1,117 @@
+Require Import Notions.
+
+
+
+Require Import Defns.
+
+Module Trivialities.
+Include Defns.Groups.
+Open Scope group_scope.
+Section top.
+Context {C : Type}.
+Variable (G: @Group C).
+
+
+Hint Resolve (closure G) ein (invin G) (linv G) (rinv G)
+             (lid G) (rid G): grp.
+Hint Rewrite @assoc : grp.
+
+Local Notation carrier := (carrier G).
+Local Notation op := (op G).
+Local Notation assoc := (assoc G).
+Local Notation e := (e G).
+Local Notation linv := (linv G).
+Local Notation rinv := (rinv G).
+Local Notation lid := (lid G).
+Local Notation rid := (rid G).
+Local Notation l_ident := (l_ident op).
+Local Notation r_ident := (r_ident op).
+
+
+
+Variable (a b c  id: C).
+Hypothesis Ga : a ∈ carrier.
+Hypothesis Gb : b ∈ carrier.
+Hypothesis Gc : c ∈ carrier.
+Hypothesis Gi : id ∈ carrier.
+Local Infix "@" := op (at level 20, left associativity).
+Local Notation "a '''" := (inv G a) (at level 2, left associativity).
+
+
+
+Theorem left_can : forall z x y, 
+  z ∈ carrier ->
+  x ∈ carrier ->
+  y ∈ carrier ->
+  z @ x = z @ y -> x = y.
+Proof with atg.
+  intros * Gz Gx Gy H.
+  rewrite <- lid, <- (lid y)...
+  rewrite <- (linv z)...
+  repeat rewrite assoc...
+  rewrite H...
+Qed.
+
+Theorem right_can : forall z x y, 
+  z ∈ carrier ->
+  x ∈ carrier ->
+  y ∈ carrier ->
+  x @ z = y @ z -> x = y.
+Proof with atg.
+  intros * Gz Gx Gy H.
+  rewrite <- rid, <- (rid y)...
+  rewrite <- (rinv z)...
+  repeat rewrite <- assoc...
+  rewrite H...
+Qed.
+
+Theorem x_is_own_inv : forall x, x ∈ carrier -> x ' ' = x.
+Proof with atg.
+  intros **. apply (left_can (x '))...
+  rewrite rinv, linv...
+Qed.
+
+Theorem id_unique : ident carrier op id -> id = e.
+Proof with atg.
+  intros H. destruct (H e)...
+  apply (left_can e)...
+  symmetry; rewrite H1...
+Qed.
+
+Theorem inv_unique : ∀ a', a' ∈ carrier -> a' @ a = e -> a @ a' = e ->
+  a' = a '.
+Proof with atg.
+  intros **. apply (left_can a)...
+  symmetry; rewrite H1...
+Qed.
+
+Theorem inv_of_op : (a @ b) ' = b ' @ a '.
+Proof with atg.
+  apply (left_can (a @ b))...
+  symmetry;
+  rewrite rinv,
+          <- assoc,
+          (assoc a),
+          rinv,
+          rid...
+Qed.
+
+
+Theorem order2__comm : ∀ (x_sq: ∀ x, x @ x = e), a @ b = b @ a.
+Proof with atg.
+  intros **. apply (left_can a), (right_can b)...
+  repeat rewrite <- assoc...
+  rewrite x_sq, lid, x_sq, (assoc (a@b))...
+Qed.
+
+Theorem unit_power__ident : ∀ x, x ∈ carrier -> x @ x = x -> ident carrier op x.
+Proof with atg.
+  intros ** y ?. split.
+  - apply (left_can x)...
+    rewrite <- assoc, H0...
+  - apply (right_can x)...
+    rewrite assoc, H0...
+Qed.
+
+End top.
+End Trivialities.
