Group Thy/Notions.v
@@ -1,0 +1,45 @@
+(* Author : CESally *)
+Require Export Setoid Ensembles Utf8.
+Reserved Notation "x @ y" (at level 20, left associativity).
+
+Delimit Scope group_scope with grp.
+Arguments In [_].
+Arguments Included [_].
+Notation "e ∈ S" := (In S e) (at level 20) : group_scope.
+Notation "A ⊆ B" := (Included A B) (at level 20) : group_scope.
+Open Scope group_scope.
+
+Module T.
+Section top.
+Context {C : Type}.
+Variable D  : Ensemble C.
+Variable op : C -> C -> C.
+Variable e  : C.
+Local Infix "@" := op (at level 20, left associativity).
+
+Definition is_assoc : Prop := ∀ x y z : C,
+  x ∈ D -> y ∈ D -> z ∈ D ->
+  x @ y @ z = x @ (y @ z).
+
+Definition l_ident : Prop := ∀ x, x ∈ D -> e @ x = x.
+Definition r_ident : Prop := ∀ x, x ∈ D -> x @ e = x.
+Definition   ident : Prop := ∀ x, x ∈ D -> e @ x = x /\ x @ e = x.
+
+Definition l_inv (inv:C -> C) : Prop := ∀ x, x ∈ D -> inv x @ x = e.
+Definition r_inv (inv:C -> C) : Prop := ∀ x, x ∈ D -> x @ inv x = e.
+
+Definition closed_u (inv: C -> C) : Prop := ∀ x,
+  x ∈ D -> (inv x) ∈ D.
+Definition closed_b : Prop := ∀ x y,
+  x ∈ D ->
+  y ∈ D -> (x @ y) ∈ D.
+
+Definition is_l_inv_of (x' x e:C) : Prop := x' @ x = e.
+Definition is_r_inv_of (x' x e:C) : Prop := x @ x' = e.
+
+Definition conjugate (h g: C) (inv: C -> C) : C := h @ g @ (inv h).
+
+End top.
+End T.
+
+Close Scope group_scope.
